\[ \mathbf{F_{11}} = \left(\begin{smallmatrix} L_{11} & 0 \\ 0 &
R_{11} \end{smallmatrix}\right) \]
\[ \mathbf{F_{12}} = \left(\begin{smallmatrix} L_{12} & 0 \\ 0 &
R_{12} \end{smallmatrix}\right) \]
\[ \mathbf{F_{21}} = \left(\begin{smallmatrix} L_{21} & 0 \\ 0 &
R_{21} \end{smallmatrix}\right) \]
\[ \mathbf{F_{22}} = \left(\begin{smallmatrix} L_{22} & 0 \\ 0 &
R_{22} \end{smallmatrix}\right) \]
\[ \mathbf{B}=\mathbf{F_{12}}^{-1}\cdot\left[ \mathbf{Sk} -
\mathbf{F_{11}} \right]  \]
\[ \mathbf{A}=\mathbf{F_{21}}+ \mathbf{F_{22}}\cdot\mathbf{B} \]
\[ \mathbf{Su} = \mathbf{B} \cdot \mathbf{A}^{-1} \]
