\[ \mathbf{Gi_{33}} = \left[\boldsymbol{\mathbbm{I}}
-\left(\begin{smallmatrix} 0 & D_{11} \\ 0 & 0
\end{smallmatrix}\right)\right]^{-1} \]
\[ \mathbf{F_{11}} = \left(\begin{smallmatrix} 1 & 0
\end{smallmatrix}\right) \cdot\mathbf{Gi_{33}}\cdot
\left(\begin{smallmatrix} 0 \\ 1 \end{smallmatrix}\right) \]
\[ \mathbf{F_{12}} = \left(\begin{smallmatrix} 1 & 0
\end{smallmatrix}\right) \cdot\mathbf{Gi_{33}}\cdot
\left(\begin{smallmatrix} D_{12} \\ 0 \end{smallmatrix}\right) \]
\[ \mathbf{F_{21}} = \left(\begin{smallmatrix} 0 & D_{21}
\end{smallmatrix}\right) \cdot\mathbf{Gi_{33}}\cdot
\left(\begin{smallmatrix} 0 \\ 1 \end{smallmatrix}\right) \]
\[ \mathbf{F_{22}} = \left(\begin{smallmatrix} 0 & D_{21}
\end{smallmatrix}\right) \cdot\mathbf{Gi_{33}}\cdot
\left(\begin{smallmatrix} D_{12} \\ 0 \end{smallmatrix}\right) +
D_{22} \]
\[ \mathbf{B}=\mathbf{F_{12}}^{-1}\cdot\left[ \mathbf{Sk} -
\mathbf{F_{11}} \right]  \]
\[ \mathbf{A}=\mathbf{F_{21}}+ \mathbf{F_{22}}\cdot\mathbf{B} \]
\[ \mathbf{Su} = \mathbf{B} \cdot \mathbf{A}^{-1} \]
